posts/approachable-language-design.md
@@ -11,3 +11,7 @@ always prefer to pass data explicitly and only proofs and types (which are reall
 
 
 the big problem with the convention of global constructors for datatype fields is that the names end up having to be mangled since they aren't scoped and could collide! it's terrible design to easily allow these unscoped operators/constructors
+
+
+
+One of the big ideas to create an approachable language is to really carefully design it to separate *hard prerequisite knowledge* from *defined knowledge*. Basically hard prerequisites are all the things someone absolutely must know in order to read or write the language, for example the syntax, primitive keywords and constructs, fundamental concepts, etc. These things can be much more terse and cryptic *because the learner has a known and prerequisite learning path to understand them* in the form of the basic language documentation. We know they'll be encountering them constantly, and we expect them to know them because we've provided such a paved path to do so, so it's okay if they're terse and efficient. The same doesn't go for things that can be defined *within* the language! Some random library shouldn't have the same power as the main language to introduce syntax or constructs, since we don't have any idea if someone will be able to track down that random library as the source of those constructs. The wall between what is primitively part of the language and what has been defined in user-land within the language should be crystal clear at all times.
