posts/what-is-rok.md
@@ -128,6 +128,9 @@ This project is seeking to solve these problems by creating a Tool, and a Commun
 focused on cryptographic code, and it isn't a new proof assistant with the intent to make formal verification go mainstream, but instead a library in an existing proof assistant meant to help crypto researchers
 however this project does in a way hint that the rok project is a good idea! it is also generic over different architectures and uses automatic verification condition generators
 
+- ivy http://microsoft.github.io/ivy/language.html
+only first order
+
 - bedrock
 Proprietary! It's essential systems like this aren't only controlled by corporations and governments.
 http://adam.chlipala.net/papers/BedrockICFP13/BedrockICFP13.pdf
